examples/wysteria/interpreter.fst
@@ -1,7 +1,7 @@
 (*--build-config
     options:--admit_fsi FStar.OrdSet --admit_fsi FStar.Seq --admit_fsi FStar.OrdMap --admit_fsi FStar.Set --admit_fsi Ffibridge --admit_fsi Runtime --admit_fsi FStar.IO --admit_fsi FStar.String --__temp_no_proj PSemantics;
     variables:CONTRIB=../../contrib;
-    other-files:classical.fst ext.fst set.fsi heap.fst st.fst all.fst seq.fsi seqproperties.fst ghost.fst listTot.fst ordset.fsi ordmap.fsi list.fst io.fsti string.fst prins.fst ast.fst ffibridge.fsi sem.fst psem.fst $CONTRIB/Platform/fst/Bytes.fst runtime.fsi print.fst ckt.fst crypto.fst
+    other-files:classical.fst ext.fst set.fsi heap.fst st.fst all.fst seq.fsi seqproperties.fst ghost.fst listTot.fst ordset.fsi ordmap.fsi list.fst io.fsti string.fst prins.fst ast.fst ffibridge.fsi sem.fst psem.fst $CONTRIB/Platform/fst/Bytes.fst runtime.fsi print.fst ckt.fst $CONTRIB/CoreCrypto/fst/CoreCrypto.fst ../crypto/sha1.fst crypto.fst
  --*)
 
 module Interpreter
@@ -193,12 +193,12 @@ type tstep_config (p:prin) = c:config{Conf.l c = Target /\
 opaque type witness_client_config (#a:Type) (x:a) = True
 
 let client_key:client_key =
-  let k = bytes_of_string "client_key" in
+  let k = Platform.Bytes.createBytes SHA1.keysize 0uy in
   assume (client_key_prop k == client_prop_t);
   k
 
 let server_key:server_key =
-  let k = bytes_of_string "server_key" in
+  let k = Platform.Bytes.createBytes SHA1.keysize 0uy in
   assume (server_key_prop k == server_prop_t);
   k
 
